lean/dk_math/DkMath/Collatz/PetalBridge/FloatWindow.lean
@@ -14,6 +14,7 @@ import DkMath.Collatz.PetalBridge.FloatWindow.PressureIncidenceBridge
 import DkMath.Collatz.PetalBridge.FloatWindow.PaymentMultiplicityBridge
 import DkMath.Collatz.PetalBridge.FloatWindow.PaymentBlockBridge
 import DkMath.Collatz.PetalBridge.FloatWindow.UniversalPaymentBlock
+import DkMath.Collatz.PetalBridge.FloatWindow.UniversalPaymentFamily
 
 #print "file: DkMath.Collatz.PetalBridge.FloatWindow"
 
